{
 "cells": [
  {
   "cell_type": "markdown",
   "metadata": {},
   "source": [
    "### Full Derivation of First- and Second-Order Energy Corrections\n",
    "\n",
    "We start with the perturbed Hamiltonian $ H = H_0 + \\lambda V $ and expand the energy $ E_n $ and wavefunction $ \\psi_n $ as power series in $ \\lambda $:\n",
    "$$\n",
    "E_n = E_n^{(0)} + \\lambda E_n^{(1)} + \\lambda^2 E_n^{(2)} + \\dots\n",
    "$$\n",
    "$$\n",
    "\\psi_n = \\psi_n^{(0)} + \\lambda \\psi_n^{(1)} + \\lambda^2 \\psi_n^{(2)} + \\dots\n",
    "$$\n",
    "\n",
    "### Substitute into the Schrödinger Equation:\n",
    "$$\n",
    "(H_0 + \\lambda V)(\\psi_n^{(0)} + \\lambda \\psi_n^{(1)} + \\lambda^2 \\psi_n^{(2)} + \\dots) = (E_n^{(0)} + \\lambda E_n^{(1)} + \\lambda^2 E_n^{(2)} + \\dots)(\\psi_n^{(0)} + \\lambda \\psi_n^{(1)} + \\lambda^2 \\psi_n^{(2)} + \\dots).\n",
    "$$\n",
    "\n",
    "### Collect Terms by Order of $ \\lambda $:\n",
    "\n",
    "#### 1. **Order $ \\lambda^0 $**:\n",
    "$$\n",
    "H_0 \\psi_n^{(0)} = E_n^{(0)} \\psi_n^{(0)}.\n",
    "$$\n",
    "\n",
    "This is the unperturbed Schrödinger equation.\n",
    "\n",
    "#### 2. **Order $ \\lambda^1 $**:\n",
    "$$\n",
    "H_0 \\psi_n^{(1)} + V \\psi_n^{(0)} = E_n^{(0)} \\psi_n^{(1)} + E_n^{(1)} \\psi_n^{(0)}.\n",
    "$$\n",
    "\n",
    "Rearrange to isolate $ \\psi_n^{(1)} $:\n",
    "$$\n",
    "(H_0 - E_n^{(0)}) \\psi_n^{(1)} = (E_n^{(1)} - V) \\psi_n^{(0)}.\n",
    "$$\n",
    "\n",
    "### Solving for $ E_n^{(1)} $:\n",
    "Project onto $ \\langle \\psi_n^{(0)} | $ to isolate the energy correction:\n",
    "$$\n",
    "\\langle \\psi_n^{(0)} | (H_0 - E_n^{(0)}) \\psi_n^{(1)} \\rangle = \\langle \\psi_n^{(0)} | (E_n^{(1)} - V) \\psi_n^{(0)} \\rangle.\n",
    "$$\n",
    "\n",
    "**Simplify Using Hermiticity**:\n",
    "$$\n",
    "0 = E_n^{(1)} - \\langle \\psi_n^{(0)} | V | \\psi_n^{(0)} \\rangle.\n",
    "$$\n",
    "\n",
    "**First-Order Energy Correction**:\n",
    "$$\n",
    "E_n^{(1)} = \\langle \\psi_n^{(0)} | V | \\psi_n^{(0)} \\rangle.\n",
    "$$\n",
    "\n",
    "### Deriving $ \\psi_n^{(1)} $:\n",
    "Return to the first-order equation:\n",
    "$$\n",
    "(H_0 - E_n^{(0)}) \\psi_n^{(1)} = -V \\psi_n^{(0)}.\n",
    "$$\n",
    "\n",
    "### Solving for $ \\psi_n^{(1)} $ in Terms of $ \\psi_m^{(0)} $:\n",
    "Expand $ \\psi_n^{(1)} $ as:\n",
    "$$\n",
    "\\psi_n^{(1)} = \\sum_{m \\neq n} \\frac{\\langle \\psi_m^{(0)} | V | \\psi_n^{(0)} \\rangle}{E_n^{(0)} - E_m^{(0)}} \\psi_m^{(0)}.\n",
    "$$\n",
    "\n",
    "### Second-Order Energy Correction:\n",
    "Start with:\n",
    "$$\n",
    "E_n^{(2)} = \\langle \\psi_n^{(0)} | V | \\psi_n^{(1)} \\rangle.\n",
    "$$\n",
    "\n",
    "Substitute $ \\psi_n^{(1)} $:\n",
    "$$\n",
    "E_n^{(2)} = \\langle \\psi_n^{(0)} | V | \\sum_{m \\neq n} \\frac{\\langle \\psi_m^{(0)} | V | \\psi_n^{(0)} \\rangle}{E_n^{(0)} - E_m^{(0)}} \\psi_m^{(0)} \\rangle.\n",
    "$$\n",
    "\n",
    "Expand the inner product:\n",
    "$$\n",
    "E_n^{(2)} = \\sum_{m \\neq n} \\frac{\\langle \\psi_n^{(0)} | V | \\psi_m^{(0)} \\rangle \\langle \\psi_m^{(0)} | V | \\psi_n^{(0)} \\rangle}{E_n^{(0)} - E_m^{(0)}}.\n",
    "$$\n",
    "\n",
    "Simplify using the fact that $ \\langle \\psi_n^{(0)} | V | \\psi_m^{(0)} \\rangle $ is the complex conjugate of $ \\langle \\psi_m^{(0)} | V | \\psi_n^{(0)} \\rangle $:\n",
    "$$\n",
    "E_n^{(2)} = \\sum_{m \\neq n} \\frac{|\\langle \\psi_m^{(0)} | V | \\psi_n^{(0)} \\rangle|^2}{E_n^{(0)} - E_m^{(0)}}.\n",
    "$$\n",
    "\n",
    "### Final Results:\n",
    "- **First-Order Energy Correction**:\n",
    "$$\n",
    "E_n^{(1)} = \\langle \\psi_n^{(0)} | V | \\psi_n^{(0)} \\rangle.\n",
    "$$\n",
    "\n",
    "- **Second-Order Energy Correction**:\n",
    "$$\n",
    "E_n^{(2)} = \\sum_{m \\neq n} \\frac{|\\langle \\psi_m^{(0)} | V | \\psi_n^{(0)} \\rangle|^2}{E_n^{(0)} - E_m^{(0)}}.\n",
    "$$\n"
   ]
  },
  {
   "cell_type": "markdown",
   "metadata": {},
   "source": [
    "### Full Derivation of First- and Second-Order Energy and Wavefunction Corrections\n",
    "\n",
    "We start with the perturbed Hamiltonian $ H = H_0 + \\lambda V $ and expand the energy $ E_n $ and wavefunction $ \\psi_n $ as power series in $ \\lambda $:\n",
    "$$\n",
    "E_n = E_n^{(0)} + \\lambda E_n^{(1)} + \\lambda^2 E_n^{(2)} + \\dots\n",
    "$$\n",
    "$$\n",
    "\\psi_n = \\psi_n^{(0)} + \\lambda \\psi_n^{(1)} + \\lambda^2 \\psi_n^{(2)} + \\dots\n",
    "$$\n",
    "\n",
    "### Substitute into the Schrödinger Equation:\n",
    "$$\n",
    "(H_0 + \\lambda V)(\\psi_n^{(0)} + \\lambda \\psi_n^{(1)} + \\lambda^2 \\psi_n^{(2)} + \\dots) = (E_n^{(0)} + \\lambda E_n^{(1)} + \\lambda^2 E_n^{(2)} + \\dots)(\\psi_n^{(0)} + \\lambda \\psi_n^{(1)} + \\lambda^2 \\psi_n^{(2)} + \\dots).\n",
    "$$\n",
    "\n",
    "### Collect Terms by Order of $ \\lambda $:\n",
    "\n",
    "#### 1. **Order $ \\lambda^0 $**:\n",
    "$$\n",
    "H_0 \\psi_n^{(0)} = E_n^{(0)} \\psi_n^{(0)}.\n",
    "$$\n",
    "\n",
    "This is the unperturbed Schrödinger equation.\n",
    "\n",
    "#### 2. **Order $ \\lambda^1 $**:\n",
    "$$\n",
    "H_0 \\psi_n^{(1)} + V \\psi_n^{(0)} = E_n^{(0)} \\psi_n^{(1)} + E_n^{(1)} \\psi_n^{(0)}.\n",
    "$$\n",
    "\n",
    "Rearrange to isolate $ \\psi_n^{(1)} $:\n",
    "$$\n",
    "(H_0 - E_n^{(0)}) \\psi_n^{(1)} = (E_n^{(1)} - V) \\psi_n^{(0)}.\n",
    "$$\n",
    "\n",
    "### Solving for $ E_n^{(1)} $:\n",
    "Project onto $ \\langle \\psi_n^{(0)} | $ to isolate the energy correction:\n",
    "$$\n",
    "\\langle \\psi_n^{(0)} | (H_0 - E_n^{(0)}) \\psi_n^{(1)} \\rangle = \\langle \\psi_n^{(0)} | (E_n^{(1)} - V) \\psi_n^{(0)} \\rangle.\n",
    "$$\n",
    "\n",
    "**Simplify Using Hermiticity**:\n",
    "$$\n",
    "0 = E_n^{(1)} - \\langle \\psi_n^{(0)} | V | \\psi_n^{(0)} \\rangle.\n",
    "$$\n",
    "\n",
    "**First-Order Energy Correction**:\n",
    "$$\n",
    "E_n^{(1)} = \\langle \\psi_n^{(0)} | V | \\psi_n^{(0)} \\rangle.\n",
    "$$\n",
    "\n",
    "### Deriving $ \\psi_n^{(1)} $:\n",
    "Return to the first-order equation:\n",
    "$$\n",
    "(H_0 - E_n^{(0)}) \\psi_n^{(1)} = -V \\psi_n^{(0)}.\n",
    "$$\n",
    "\n",
    "### Solving for $ \\psi_n^{(1)} $ in Terms of $ \\psi_m^{(0)} $:\n",
    "Expand $ \\psi_n^{(1)} $ as:\n",
    "$$\n",
    "\\psi_n^{(1)} = \\sum_{m \\neq n} c_m \\psi_m^{(0)},\n",
    "$$\n",
    "where\n",
    "$$\n",
    "c_m = \\frac{\\langle \\psi_m^{(0)} | V | \\psi_n^{(0)} \\rangle}{E_n^{(0)} - E_m^{(0)}}.\n",
    "$$\n",
    "\n",
    "Substitute this into $ \\psi_n^{(1)} $:\n",
    "$$\n",
    "\\psi_n^{(1)} = \\sum_{m \\neq n} \\frac{\\langle \\psi_m^{(0)} | V | \\psi_n^{(0)} \\rangle}{E_n^{(0)} - E_m^{(0)}} \\psi_m^{(0)}.\n",
    "$$\n",
    "\n",
    "### Second-Order Energy Correction:\n",
    "Start with:\n",
    "$$\n",
    "E_n^{(2)} = \\langle \\psi_n^{(0)} | V | \\psi_n^{(1)} \\rangle.\n",
    "$$\n",
    "\n",
    "Substitute $ \\psi_n^{(1)} $:\n",
    "$$\n",
    "E_n^{(2)} = \\langle \\psi_n^{(0)} | V | \\sum_{m \\neq n} \\frac{\\langle \\psi_m^{(0)} | V | \\psi_n^{(0)} \\rangle}{E_n^{(0)} - E_m^{(0)}} \\psi_m^{(0)} \\rangle.\n",
    "$$\n",
    "\n",
    "Expand the inner product:\n",
    "$$\n",
    "E_n^{(2)} = \\sum_{m \\neq n} \\frac{\\langle \\psi_n^{(0)} | V | \\psi_m^{(0)} \\rangle \\langle \\psi_m^{(0)} | V | \\psi_n^{(0)} \\rangle}{E_n^{(0)} - E_m^{(0)}}.\n",
    "$$\n",
    "\n",
    "Simplify using the fact that $ \\langle \\psi_n^{(0)} | V | \\psi_m^{(0)} \\rangle $ is the complex conjugate of $ \\langle \\psi_m^{(0)} | V | \\psi_n^{(0)} \\rangle $:\n",
    "$$\n",
    "E_n^{(2)} = \\sum_{m \\neq n} \\frac{|\\langle \\psi_m^{(0)} | V | \\psi_n^{(0)} \\rangle|^2}{E_n^{(0)} - E_m^{(0)}}.\n",
    "$$\n",
    "\n",
    "### Deriving $ \\psi_n^{(2)} $:\n",
    "To find the second-order correction $ \\psi_n^{(2)} $, we start with the second-order equation:\n",
    "$$\n",
    "H_0 \\psi_n^{(2)} + V \\psi_n^{(1)} = E_n^{(0)} \\psi_n^{(2)} + E_n^{(1)} \\psi_n^{(1)} + E_n^{(2)} \\psi_n^{(0)}.\n",
    "$$\n",
    "\n",
    "Rearrange:\n",
    "$$\n",
    "(H_0 - E_n^{(0)}) \\psi_n^{(2)} = -V \\psi_n^{(1)} + E_n^{(1)} \\psi_n^{(1)} + E_n^{(2)} \\psi_n^{(0)}.\n",
    "$$\n",
    "\n",
    "Substitute $ E_n^{(1)} = \\langle \\psi_n^{(0)} | V | \\psi_n^{(0)} \\rangle $ and expand $ \\psi_n^{(1)} $ using the known expression:\n",
    "$$\n",
    "\\psi_n^{(2)} = \\sum_{k \\neq n} \\frac{\\langle \\psi_k^{(0)} | V | \\psi_n^{(1)} \\rangle}{E_n^{(0)} - E_k^{(0)}} \\psi_k^{(0)}.\n",
    "$$\n",
    "\n",
    "### Final Results:\n",
    "- **First-Order Energy Correction**:\n",
    "$$\n",
    "E_n^{(1)} = \\langle \\psi_n^{(0)} | V | \\psi_n^{(0)} \\rangle.\n",
    "$$\n",
    "\n",
    "- **Second-Order Energy Correction**:\n",
    "$$\n",
    "E_n^{(2)} = \\sum_{m \\neq n} \\frac{|\\langle \\psi_m^{(0)} | V | \\psi_n^{(0)} \\rangle|^2}{E_n^{(0)} - E_m^{(0)}}.\n",
    "$$\n",
    "\n",
    "- **First-Order Wavefunction Correction**:\n",
    "$$\n",
    "\\psi_n^{(1)} = \\sum_{m \\neq n} \\frac{\\langle \\psi_m^{(0)} | V | \\psi_n^{(0)} \\rangle}{E_n^{(0)} - E_m^{(0)}} \\psi_m^{(0)}.\n",
    "$$\n",
    "\n",
    "- **Second-Order Wavefunction Correction**:\n",
    "$$\n",
    "\\psi_n^{(2)} = \\sum_{k \\neq n} \\frac{\\langle \\psi_k^{(0)} | V | \\psi_n^{(1)} \\rangle}{E_n^{(0)} - E_k^{(0)}} \\psi_k^{(0)}.\n",
    "$$\n"
   ]
  },
  {
   "cell_type": "markdown",
   "metadata": {},
   "source": []
  }
 ],
 "metadata": {
  "language_info": {
   "name": "python"
  }
 },
 "nbformat": 4,
 "nbformat_minor": 2
}
